ModularEngine/src/LogicEngine.FStar/prims.fst
@@ -215,6 +215,7 @@ extern Runtime val intToString: n:int -> s:string{s=(ReprInt n)}
 extern Runtime val stringToInt: s:string -> n:int{s=(ReprInt n)}
 extern Runtime val strRmPfx: s:string -> pfx:string -> r:string{s=(Strcat pfx r)}
 extern Runtime val strSplitByDelimiter: s:string -> d:string -> (r1:string*r2:string{(Strcat r1 r2)=s})
+extern Runtime val intCheckRange: int -> int -> int -> bool
 
 extern Runtime val boxToObject: 'a -> object
 extern Runtime val addBindings: object -> string -> bool
